Consolidate context store modules

ContextStore/StoreCore.v
@@ -1,6 +1,6 @@
 (** * Generic stores: core definitions *)
 
-From ContextBase Require Import Prelude LogicVar.
+From ContextBase Require Import Prelude LogicVar BaseTactics.
 From Stdlib Require Import Logic.ProofIrrelevance.
 
 Section AbstractStoreCore.
@@ -49,7 +49,7 @@ Definition storeA_rekey {K : Type} `{Countable K}
     (f : K → K) (s : StoreA K) : StoreA K :=
   storeA_map_key f s.
 
-Definition storeA_swap {K : Type} `{Countable K} 
+Definition storeA_swap {K : Type} `{Countable K}
     (x y : K) (s : StoreA K) : StoreA K :=
   storeA_rekey (swap x y) s.
 
@@ -155,3 +155,666 @@ End AbstractStoreCore.
 
 Arguments storeAO_store {_ _ _ _ _} _.
 Arguments storeAO_dom {_ _ _ _ _} _.
+
+(** ** Generic stores: key actions *)
+
+Section AbstractStoreCore.
+
+Context {V : Type} `{ValueSig V}.
+
+Lemma storeA_rekey_lookup {K : Type} `{Countable K}
+    (f : K → K) (Hf : Inj (=) (=) f) (s : StoreA K) (z : K) :
+  ((storeA_rekey f s : gmap K V) !! f z) =
+  ((s : gmap K V) !! z).
+Proof.
+  unfold storeA_rekey, storeA_map_key.
+  change (kmap (M2:=gmap K) f s !! f z = s !! z).
+  rewrite (lookup_kmap (M1:=gmap K) (M2:=gmap K)
+    (Inj0:=Hf) f s z).
+  reflexivity.
+Qed.
+
+Lemma storeA_rekey_dom {K : Type} `{Countable K}
+    (f : K → K) (Hf : Inj (=) (=) f) (s : StoreA K) :
+  dom (storeA_rekey f s : gmap K V) = set_map f (dom (s : gmap K V)).
+Proof.
+  unfold storeA_rekey, storeA_map_key.
+  change (dom (kmap (M2:=gmap K) f s) =
+    set_map f (dom (s : gmap K V))).
+  rewrite (dom_kmap_L (M:=gmap K) (M2:=gmap K)
+    (Inj0:=Hf) f (s : gmap K V)).
+  reflexivity.
+Qed.
+
+Definition storeA_rekey_inj_on_dom {K : Type} `{Countable K}
+    (f : K → K) (s : StoreA K) : Prop :=
+  forall x y,
+    x ∈ dom (s : gmap K V) ->
+    y ∈ dom (s : gmap K V) ->
+    f x = f y ->
+    x = y.
+
+Lemma storeA_rekey_mapped_fst_nodup {K : Type} `{Countable K}
+    (f : K → K) (s : StoreA K) :
+  storeA_rekey_inj_on_dom f s ->
+  NoDup ((prod_map f id <$> map_to_list (s : gmap K V)).*1).
+Proof.
+  intros Hinj.
+  replace ((prod_map f id <$> map_to_list (s : gmap K V)).*1)
+    with ((fun p : K * V => f p.1) <$> map_to_list (s : gmap K V)).
+  2:{
+    induction (map_to_list (s : gmap K V)) as [|[x v] l IH];
+      simpl; [reflexivity|].
+    f_equal. exact IH.
+  }
+  apply NoDup_fmap_2_strong.
+  - intros [x vx] [y vy] Hx Hy Heq. simpl in Heq.
+    assert (Hxy : x = y).
+    {
+      apply Hinj.
+      - apply elem_of_dom. exists vx. rewrite <- elem_of_map_to_list. exact Hx.
+      - apply elem_of_dom. exists vy. rewrite <- elem_of_map_to_list. exact Hy.
+      - exact Heq.
+    }
+    subst y.
+    assert (vx = vy).
+    {
+      rewrite elem_of_map_to_list in Hx.
+      rewrite elem_of_map_to_list in Hy.
+      rewrite Hx in Hy. inversion Hy. reflexivity.
+    }
+    subst vy. reflexivity.
+  - apply NoDup_map_to_list.
+Qed.
+
+Lemma storeA_rekey_lookup_Some_inj_on {K : Type} `{Countable K}
+    (f : K → K) (s : StoreA K) (z : K) (v : V) :
+  storeA_rekey_inj_on_dom f s ->
+  ((storeA_rekey f s : gmap K V) !! z = Some v <->
+    exists x, z = f x /\ (s : gmap K V) !! x = Some v).
+Proof.
+  intros Hinj.
+  unfold storeA_rekey, storeA_map_key, kmap.
+  rewrite <- elem_of_list_to_map.
+  - rewrite list_elem_of_fmap.
+    split.
+    + intros [[x vx] [Hz Hv]]. simpl in Hz. inversion Hz. subst.
+      rewrite elem_of_map_to_list in Hv.
+      exists x. split; [reflexivity|exact Hv].
+    + intros [x [Hz Hx]]. exists (x, v). split.
+      * subst z. reflexivity.
+      * rewrite elem_of_map_to_list. exact Hx.
+  - apply storeA_rekey_mapped_fst_nodup. exact Hinj.
+Qed.
+
+Lemma storeA_rekey_lookup_None_inj_on {K : Type} `{Countable K}
+    (f : K → K) (s : StoreA K) (z : K) :
+  storeA_rekey_inj_on_dom f s ->
+  ((storeA_rekey f s : gmap K V) !! z = None <->
+    forall x, z = f x -> (s : gmap K V) !! x = None).
+Proof.
+  intros Hinj.
+  rewrite <- !not_elem_of_dom.
+  split.
+  - intros Hnone x Hz.
+    apply not_elem_of_dom. intros Hx.
+    apply Hnone. apply elem_of_dom in Hx as [v Hv].
+    apply elem_of_dom. exists v.
+    apply storeA_rekey_lookup_Some_inj_on; [exact Hinj|].
+    exists x. split; [exact Hz|exact Hv].
+  - intros Hnone Hz.
+    apply elem_of_dom in Hz as [v Hv].
+    apply storeA_rekey_lookup_Some_inj_on in Hv as [x [Hz Hx]];
+      [|exact Hinj].
+    rewrite (Hnone x Hz) in Hx. discriminate.
+Qed.
+
+Lemma storeA_rekey_dom_inj_on {K : Type} `{Countable K}
+    (f : K → K) (s : StoreA K) :
+  storeA_rekey_inj_on_dom f s ->
+  dom (storeA_rekey f s : gmap K V) = set_map f (dom (s : gmap K V)).
+Proof.
+  intros Hinj.
+  apply set_eq. intros z.
+  rewrite elem_of_dom, elem_of_map.
+  split.
+  - intros [v Hv].
+    apply storeA_rekey_lookup_Some_inj_on in Hv as [x [Hz Hx]];
+      [|exact Hinj].
+    exists x. split; [exact Hz|].
+    apply elem_of_dom. exists v. exact Hx.
+  - intros [x [Hz Hx]].
+    apply elem_of_dom in Hx as [v Hv].
+    exists v.
+    apply storeA_rekey_lookup_Some_inj_on; [exact Hinj|].
+    exists x. split; [exact Hz|exact Hv].
+Qed.
+
+Lemma storeA_rekey_lookup_none_inj_on {K : Type} `{Countable K}
+    (f : K → K) (s : StoreA K) (x : K) :
+  (s : gmap K V) !! x = None ->
+  (forall y,
+      y ∈ dom (s : gmap K V) ->
+      f y <> f x) ->
+  (storeA_rekey f s : gmap K V) !! f x = None.
+Proof.
+  intros Hnone Hfresh.
+  apply not_elem_of_dom. intros Hin.
+  apply elem_of_dom in Hin as [v Hv].
+  unfold storeA_rekey, storeA_map_key, kmap in Hv.
+  apply elem_of_list_to_map_2 in Hv.
+  apply list_elem_of_fmap in Hv as [[y vy] [Hy Hlook]].
+  simpl in Hy. injection Hy as Hkey Hval. subst vy.
+  rewrite elem_of_map_to_list in Hlook.
+  apply (Hfresh y); [apply elem_of_dom; eauto|symmetry; exact Hkey].
+Qed.
+
+Lemma storeA_rekey_insert_inj_on {K : Type} `{Countable K}
+    (f : K → K) z v (s : StoreA K) :
+  (s : gmap K V) !! z = None ->
+  storeA_rekey_inj_on_dom f (<[z := v]> (s : gmap K V)) ->
+  storeA_rekey f (<[z := v]> s) =
+  <[f z := v]> (storeA_rekey f s : gmap K V).
+Proof.
+  intros Hnone Hinj.
+  apply storeA_map_eq. intros y.
+  change (((storeA_rekey f (<[z := v]> s) : gmap K V) !! y) =
+    ((<[f z := v]> (storeA_rekey f s : gmap K V)) !! y)).
+  destruct (decide (y = f z)) as [->|Hy].
+  - rewrite lookup_insert_eq.
+    apply storeA_rekey_lookup_Some_inj_on.
+    + exact Hinj.
+    + exists z. split; [reflexivity|].
+      change ((<[z := v]> (s : gmap K V)) !! z = Some v).
+      rewrite lookup_insert_eq. reflexivity.
+  - rewrite lookup_insert_ne by (intros Heq; apply Hy; symmetry; exact Heq).
+    destruct ((storeA_rekey f s : gmap K V) !! y) as [w|] eqn:Hylook.
+    + apply storeA_rekey_lookup_Some_inj_on.
+      * exact Hinj.
+      * apply storeA_rekey_lookup_Some_inj_on in Hylook as [x [Hyx Hx]].
+        -- exists x. split; [exact Hyx|].
+           change ((<[z := v]> (s : gmap K V)) !! x = Some w).
+           rewrite lookup_insert_ne.
+           ++ exact Hx.
+           ++ intros ->. apply Hy. exact Hyx.
+        -- intros a b Ha Hb Hab.
+           apply Hinj.
+           ++ change (a ∈ dom (<[z := v]> (s : gmap K V))).
+              rewrite dom_insert_L. apply elem_of_union_r. exact Ha.
+           ++ change (b ∈ dom (<[z := v]> (s : gmap K V))).
+              rewrite dom_insert_L. apply elem_of_union_r. exact Hb.
+           ++ exact Hab.
+    + apply storeA_rekey_lookup_None_inj_on.
+      * exact Hinj.
+      * intros x Hyx.
+        destruct (decide (x = z)) as [->|Hxz].
+        -- exfalso. apply Hy. exact Hyx.
+        -- change ((<[z := v]> (s : gmap K V)) !! x = None).
+           rewrite lookup_insert_ne by (intros Heq; apply Hxz; symmetry; exact Heq).
+           assert (Hinj_s : storeA_rekey_inj_on_dom f s).
+           {
+             intros a b Ha Hb Hab.
+              apply Hinj.
+              ** change (a ∈ dom (<[z := v]> (s : gmap K V))).
+                 rewrite dom_insert_L. apply elem_of_union_r. exact Ha.
+              ** change (b ∈ dom (<[z := v]> (s : gmap K V))).
+                 rewrite dom_insert_L. apply elem_of_union_r. exact Hb.
+              ** exact Hab.
+           }
+           pose proof (storeA_rekey_lookup_None_inj_on f s y Hinj_s)
+             as [Hto _].
+           exact (Hto Hylook x Hyx).
+Qed.
+
+Lemma storeA_rekey_ext_on_dom {K : Type} `{Countable K}
+    (f g : K → K) (s : StoreA K) :
+  (forall x, x ∈ dom (s : gmap K V) -> f x = g x) ->
+  storeA_rekey f s = storeA_rekey g s.
+Proof.
+  intros Hext.
+  unfold storeA_rekey, storeA_map_key, kmap.
+  f_equal.
+  set (l := map_to_list (s : gmap K V)).
+  assert (Hdom : forall x v, (x, v) ∈ l -> x ∈ dom (s : gmap K V)).
+  {
+    subst l. intros x v Hin.
+    apply elem_of_dom. exists v.
+    rewrite <- elem_of_map_to_list. exact Hin.
+  }
+  clearbody l.
+  induction l as [|[x v] l IH]; simpl; [reflexivity|].
+  f_equal.
+  - simpl. rewrite Hext by (apply (Hdom x v); left; reflexivity).
+    reflexivity.
+  - apply IH. intros y w Hin.
+    apply (Hdom y w). right. exact Hin.
+Qed.
+
+Lemma storeA_rekey_compose_inj_on {K : Type} `{Countable K}
+    (f g : K → K) (s : StoreA K) :
+  storeA_rekey_inj_on_dom g s ->
+  storeA_rekey_inj_on_dom f (storeA_rekey g s) ->
+  storeA_rekey f (storeA_rekey g s) =
+  storeA_rekey (fun x => f (g x)) s.
+Proof.
+  intros Hg Hf.
+  assert (Hcomp : storeA_rekey_inj_on_dom (fun x => f (g x)) s).
+  {
+    intros x y Hx Hy Heq.
+    apply Hg; [exact Hx|exact Hy|].
+    apply Hf.
+    - rewrite storeA_rekey_dom_inj_on by exact Hg.
+      apply elem_of_map. exists x. split; [reflexivity|exact Hx].
+    - rewrite storeA_rekey_dom_inj_on by exact Hg.
+      apply elem_of_map. exists y. split; [reflexivity|exact Hy].
+    - exact Heq.
+  }
+  apply storeA_map_eq. intros z.
+  change (((storeA_rekey f (storeA_rekey g s) : gmap K V) !! z) =
+    ((storeA_rekey (fun x => f (g x)) s : gmap K V) !! z)).
+  destruct ((storeA_rekey f (storeA_rekey g s) : gmap K V) !! z)
+    as [v|] eqn:HL.
+  - apply storeA_rekey_lookup_Some_inj_on in HL as [y [Hz Hy]];
+      [|exact Hf].
+    apply storeA_rekey_lookup_Some_inj_on in Hy as [x [Hy Hx]];
+      [|exact Hg].
+    symmetry. apply storeA_rekey_lookup_Some_inj_on; [exact Hcomp|].
+    subst y. exists x. split; [exact Hz|exact Hx].
+  - destruct ((storeA_rekey (fun x => f (g x)) s : gmap K V) !! z)
+      as [v|] eqn:HR; [|reflexivity].
+    exfalso.
+    apply storeA_rekey_lookup_Some_inj_on in HR as [x [Hz Hx]];
+      [|exact Hcomp].
+    assert (Hgx : (storeA_rekey g s : gmap K V) !! g x = Some v).
+    {
+      apply storeA_rekey_lookup_Some_inj_on; [exact Hg|].
+      exists x. split; [reflexivity|exact Hx].
+    }
+    assert (HLsome :
+      (storeA_rekey f (storeA_rekey g s) : gmap K V) !! z = Some v).
+    {
+      apply storeA_rekey_lookup_Some_inj_on; [exact Hf|].
+      exists (g x). split; [exact Hz|exact Hgx].
+    }
+    rewrite HL in HLsome. discriminate.
+Qed.
+
+Lemma storeA_rekey_compose {K : Type} `{Countable K}
+    (f g : K → K) (Hf : Inj (=) (=) f) (Hg : Inj (=) (=) g)
+    (s : StoreA K) :
+  storeA_rekey (V:=V) (K:=K) f (storeA_rekey (V:=V) (K:=K) g s) =
+  storeA_rekey (V:=V) (K:=K) (fun x => f (g x)) s.
+Proof.
+  apply storeA_rekey_compose_inj_on.
+  - intros a b _ _ Hab. apply Hg. exact Hab.
+  - intros a b _ _ Hab. apply Hf. exact Hab.
+Qed.
+
+Definition storeA_on_rekey {K : Type} `{Countable K}
+    (f : K → K) (Hf : Inj (=) (=) f)
+    {D : gset K} (s : StoreAOn (V:=V) D) : StoreAOn (V:=V) (set_map f D).
+Proof.
+  destruct s as [s Hdom].
+  refine {| storeAO_store := storeA_rekey f s |}.
+  change (dom (storeA_rekey f s : gmap K V) = set_map f D).
+  rewrite storeA_rekey_dom by exact Hf.
+  replace (dom (s : gmap K V)) with D by (symmetry; exact Hdom).
+  reflexivity.
+Defined.
+
+Lemma storeA_rekey_empty {K : Type} `{Countable K}
+    (f : K → K) :
+  storeA_rekey f (∅ : StoreA K) = (∅ : gmap K V).
+Proof.
+  unfold storeA_rekey, storeA_map_key.
+  change (kmap (M2:=gmap K) f (∅ : gmap K V) =
+    (∅ : gmap K V)).
+  apply kmap_empty.
+Qed.
+
+Lemma storeA_rekey_insert {K : Type} `{Countable K}
+    (f : K → K) (Hf : Inj (=) (=) f) z v (s : StoreA K) :
+  storeA_rekey f (<[z := v]> s) =
+  <[f z := v]> (storeA_rekey f s : gmap K V).
+Proof.
+  unfold storeA_rekey, storeA_map_key.
+  change (kmap f (<[z := v]> (s : gmap K V)) =
+    (<[f z := v]> (kmap f (s : gmap K V)) : gmap K V)).
+  refine (@kmap_insert K (gmap K) _ _ _ _ _ _ _ _ _
+    K (gmap K) _ _ _ _ _ _ _ _ _
+    f _ V (s : gmap K V) z v).
+Qed.
+
+Lemma storeA_rekey_delete {K : Type} `{Countable K}
+    (f : K → K) (Hf : Inj (=) (=) f) z (s : StoreA K) :
+  storeA_rekey f (delete z s) =
+  delete (f z) (storeA_rekey f s : gmap K V).
+Proof.
+  unfold storeA_rekey, storeA_map_key.
+  change (kmap (M2:=gmap K) f (delete z (s : gmap K V)) =
+    delete (f z) (kmap (M2:=gmap K) f (s : gmap K V))).
+  refine (@kmap_delete K (gmap K) _ _ _ _ _ _ _ _ _
+    K (gmap K) _ _ _ _ _ _ _ _ _
+    f _ V (s : gmap K V) z).
+Qed.
+
+Lemma storeA_rekey_union {K : Type} `{Countable K}
+    (f : K → K) (Hf : Inj (=) (=) f) (s1 s2 : StoreA K) :
+  storeA_rekey f (@union (gmap K V) _ s1 s2) =
+  @union (gmap K V) _
+    (storeA_rekey f s1 : gmap K V) (storeA_rekey f s2 : gmap K V).
+Proof.
+  unfold storeA_rekey, storeA_map_key.
+  change (kmap f (@union (gmap K V) _ (s1 : gmap K V) (s2 : gmap K V)) =
+    @union (gmap K V) _
+      (kmap f (s1 : gmap K V))
+      (kmap f (s2 : gmap K V))).
+  refine (@kmap_union K (gmap K) _ _ _ _ _ _ _ _ _
+    K (gmap K) _ _ _ _ _ _ _ _ _
+    f _ V (s1 : gmap K V) (s2 : gmap K V)).
+Qed.
+
+Lemma storeA_map_key_lookup {K K' : Type} `{Countable K} `{Countable K'}
+    (f : K → K') (Hf : Inj (=) (=) f) (s : StoreA K) (z : K) :
+  ((storeA_map_key f s : gmap K' V) !! f z) =
+  ((s : gmap K V) !! z).
+Proof.
+  unfold storeA_map_key.
+  change (kmap (M1:=gmap K) (M2:=gmap K') f s !! f z = s !! z).
+  rewrite (lookup_kmap (M1:=gmap K) (M2:=gmap K')
+    (Inj0:=Hf) f s z).
+  reflexivity.
+Qed.
+
+Lemma storeA_map_key_dom {K K' : Type} `{Countable K} `{Countable K'}
+    (f : K → K') (Hf : Inj (=) (=) f) (s : StoreA K) :
+  dom (storeA_map_key f s : gmap K' V) = set_map f (dom (s : gmap K V)).
+Proof.
+  unfold storeA_map_key.
+  change (dom (kmap (M1:=gmap K) (M2:=gmap K') f s) =
+    set_map f (dom (s : gmap K V))).
+  rewrite (dom_kmap_L (M:=gmap K) (M2:=gmap K')
+    (Inj0:=Hf) f (s : gmap K V)).
+  reflexivity.
+Qed.
+
+Lemma storeA_map_key_insert {K K' : Type} `{Countable K} `{Countable K'}
+    (f : K → K') (Hf : Inj (=) (=) f) z v (s : StoreA K) :
+  storeA_map_key f (<[z := v]> s) =
+  <[f z := v]> (storeA_map_key f s : gmap K' V).
+Proof.
+  unfold storeA_map_key.
+  change (kmap f (<[z := v]> (s : gmap K V)) =
+    (<[f z := v]> (kmap f (s : gmap K V)) : gmap K' V)).
+  refine (@kmap_insert K (gmap K) _ _ _ _ _ _ _ _ _
+    K' (gmap K') _ _ _ _ _ _ _ _ _
+    f _ V (s : gmap K V) z v).
+Qed.
+
+Lemma storeA_on_rekey_id_on_dom {K : Type} `{Countable K}
+    (f : K → K) (Hf : Inj (=) (=) f)
+    (D : gset K) (s : StoreAOn (V:=V) D) :
+  (forall x, x ∈ D -> f x = x) ->
+  storeAO_store (storeA_on_rekey f Hf s) = storeAO_store s.
+Proof.
+  intros Hid.
+  destruct s as [s Hdom]. cbn [storeAO_store storeA_on_rekey].
+  apply (map_eq (M:=gmap K)). intros z.
+  destruct ((s : gmap K V) !! z) as [v|] eqn:Hz.
+  - assert (HzD : z ∈ D).
+    { rewrite <- Hdom. by apply elem_of_dom_2 in Hz. }
+    rewrite <- (Hid z HzD) at 1.
+    rewrite storeA_rekey_lookup by exact Hf. exact Hz.
+  - destruct ((storeA_rekey f s : gmap K V) !! z) as [v|] eqn:Hzr;
+      [|reflexivity].
+    exfalso.
+    assert (Hzdom : z ∈ dom (storeA_rekey f s : gmap K V)).
+    { by apply elem_of_dom_2 in Hzr. }
+    rewrite storeA_rekey_dom in Hzdom by exact Hf.
+    apply elem_of_map in Hzdom as [u [Hzu HuD]].
+    assert (HuD' : u ∈ D).
+    { rewrite <- Hdom. exact HuD. }
+    rewrite Hid in Hzu by exact HuD'. subst z.
+    change (u ∈ dom (s : gmap K V)) in HuD.
+    apply elem_of_dom in HuD as [w Hw]. congruence.
+Qed.
+
+End AbstractStoreCore.
+
+Section AbstractStoreCore.
+
+Context {V : Type} `{ValueSig V}.
+
+Lemma storeA_swap_lookup {K : Type} `{Countable K}
+    (x y : K) (s : StoreA K) (z : K) :
+  ((@storeA_swap V K _ _ x y s : gmap K V) !! swap x y z) =
+  ((s : gmap K V) !! z).
+Proof.
+  unfold storeA_swap.
+  change (kmap (M2:=gmap K) (swap x y) s !! swap x y z = s !! z).
+  pose proof (swap_inj x y) as Hinj.
+  rewrite (lookup_kmap (M1:=gmap K) (M2:=gmap K)
+    (Inj0:=Hinj) (swap x y) s z).
+  reflexivity.
+Qed.
+
+Lemma storeA_swap_lookup_inv {K : Type} `{Countable K}
+    (x y : K) (s : StoreA K) (z : K) :
+  ((@storeA_swap V K _ _ x y s : gmap K V) !! z) =
+  ((s : gmap K V) !! swap x y z).
+Proof.
+  rewrite <- (swap_involutive x y z) at 1.
+  apply storeA_swap_lookup.
+Qed.
+
+Lemma storeA_swap_dom {K : Type} `{Countable K}
+    (x y : K) (s : StoreA K) :
+  dom (@storeA_swap V K _ _ x y s : gmap K V) =
+  set_swap x y (dom (s : gmap K V)).
+Proof.
+  unfold storeA_swap, set_swap.
+  change (dom (kmap (M2:=gmap K) (swap x y) s) =
+    set_map (swap x y) (dom s)).
+  pose proof (swap_inj x y) as Hinj.
+  rewrite (dom_kmap_L (M:=gmap K) (M2:=gmap K)
+    (Inj0:=Hinj) (swap x y) s).
+  reflexivity.
+Qed.
+
+Lemma storeA_swap_delete {K : Type} `{Countable K}
+    (x y z : K) (s : StoreA K) :
+   @storeA_swap V K _ _ x y (delete z s) =
+  delete (swap x y z) (@storeA_swap V K _ _ x y s : gmap K V).
+Proof.
+  unfold storeA_swap.
+  change (kmap (M2:=gmap K) (swap x y) (delete z (s : gmap K V)) =
+    delete (swap x y z)
+      (kmap (M2:=gmap K) (swap x y) (s : gmap K V))).
+  refine (@kmap_delete K (gmap K) _ _ _ _ _ _ _ _ _
+    K (gmap K) _ _ _ _ _ _ _ _ _
+    (swap x y) _ V (s : gmap K V) z).
+  apply swap_inj.
+Qed.
+
+Lemma storeA_swap_insert {K : Type} `{Countable K}
+    (x y z : K) (v : V) (s : StoreA K) :
+   @storeA_swap V K _ _ x y (<[z := v]> s) =
+  <[swap x y z := v]> (@storeA_swap V K _ _ x y s : gmap K V).
+Proof.
+  unfold storeA_swap.
+  change (kmap (swap x y) (<[z := v]> (s : gmap K V)) =
+    (<[swap x y z := v]>
+      (kmap (swap x y) (s : gmap K V)) : gmap K V)).
+  refine (@kmap_insert K (gmap K) _ _ _ _ _ _ _ _ _
+    K (gmap K) _ _ _ _ _ _ _ _ _
+    (swap x y) _ V (s : gmap K V) z v).
+  apply swap_inj.
+Qed.
+
+Lemma storeA_swap_union {K : Type} `{Countable K}
+    (x y : K) (s1 s2 : StoreA K) :
+   @storeA_swap V K _ _ x y (@union (gmap K V) _ s1 s2) =
+  @union (gmap K V) _ (@storeA_swap V K _ _ x y s1 : gmap K V) (@storeA_swap V K _ _ x y s2 : gmap K V).
+Proof.
+  unfold storeA_swap.
+  change (kmap (swap x y) (@union (gmap K V) _ (s1 : gmap K V) (s2 : gmap K V)) =
+    @union (gmap K V) _
+      (kmap (swap x y) (s1 : gmap K V))
+      (kmap (swap x y) (s2 : gmap K V))).
+  refine (@kmap_union K (gmap K) _ _ _ _ _ _ _ _ _
+    K (gmap K) _ _ _ _ _ _ _ _ _
+    (swap x y) _ V (s1 : gmap K V) (s2 : gmap K V)).
+  apply swap_inj.
+Qed.
+
+Lemma storeA_swap_involutive {K : Type} `{Countable K}
+    (x y : K) (s : StoreA K) :
+   @storeA_swap V K _ _ x y (@storeA_swap V K _ _ x y s : StoreA K) = s.
+Proof.
+  apply storeA_map_eq. intros z.
+  change (((@storeA_swap V K _ _ x y
+    (@storeA_swap V K _ _ x y s) : gmap K V) !! z) =
+    ((s : gmap K V) !! z)).
+  rewrite storeA_swap_lookup_inv, storeA_swap_lookup_inv.
+  better_base_solver.
+Qed.
+
+Lemma storeA_swap_sym {K : Type} `{Countable K}
+    (x y : K) (s : StoreA K) :
+   @storeA_swap V K _ _ x y s =  @storeA_swap V K _ _ y x s.
+Proof.
+  apply storeA_map_eq. intros z.
+  change (((@storeA_swap V K _ _ x y s : gmap K V) !! z) =
+    ((@storeA_swap V K _ _ y x s : gmap K V) !! z)).
+  rewrite !storeA_swap_lookup_inv.
+  rewrite swap_sym. reflexivity.
+Qed.
+
+Lemma storeA_swap_fresh {K : Type} `{Countable K}
+    (x y : K) (s : StoreA K) :
+  x ∉ dom (s : gmap K V) ->
+  y ∉ dom (s : gmap K V) ->
+   @storeA_swap V K _ _ x y s = s.
+Proof.
+  intros Hx Hy. apply storeA_map_eq. intros z.
+  change (((@storeA_swap V K _ _ x y s : gmap K V) !! z) =
+    ((s : gmap K V) !! z)).
+  rewrite storeA_swap_lookup_inv.
+  destruct (decide (z = x)) as [->|Hzx].
+	  - base_swap_normalize.
+	    change (((s : gmap K V) !! y) = ((s : gmap K V) !! x)).
+    assert (Hsx : (s : gmap K V) !! x = None) by better_map_solver.
+    assert (Hsy : (s : gmap K V) !! y = None) by better_map_solver.
+    change (((s : gmap K V) !! x) = None) in Hsx.
+    change (((s : gmap K V) !! y) = None) in Hsy.
+    rewrite Hsx, Hsy.
+    reflexivity.
+	  - destruct (decide (z = y)) as [->|Hzy].
+	    + base_swap_normalize.
+	      change (((s : gmap K V) !! x) = ((s : gmap K V) !! y)).
+      assert (Hsx : (s : gmap K V) !! x = None) by better_map_solver.
+      assert (Hsy : (s : gmap K V) !! y = None) by better_map_solver.
+      change (((s : gmap K V) !! x) = None) in Hsx.
+      change (((s : gmap K V) !! y) = None) in Hsy.
+      rewrite Hsx, Hsy.
+      reflexivity.
+	    + better_base_solver.
+Qed.
+
+Lemma storeA_swap_conjugate {K : Type} `{Countable K}
+    (a b x y : K) (s : StoreA K) :
+   @storeA_swap V K _ _ a b (@storeA_swap V K _ _ x y s : StoreA K) =
+   @storeA_swap V K _ _ (swap a b x) (swap a b y)
+    (@storeA_swap V K _ _ a b s : StoreA K).
+Proof.
+  apply storeA_map_eq. intros z.
+  change (((@storeA_swap V K _ _ a b
+    (@storeA_swap V K _ _ x y s) : gmap K V) !! z) =
+    ((@storeA_swap V K _ _ (swap a b x) (swap a b y)
+      (@storeA_swap V K _ _ a b s) : gmap K V) !! z)).
+  rewrite !storeA_swap_lookup_inv.
+  rewrite swap_conjugate_inv. reflexivity.
+Qed.
+
+Lemma storeA_swap_commute_fresh {K : Type} `{Countable K}
+    (a b c d : K) (s : StoreA K) :
+  c <> a ->
+  c <> b ->
+  d <> a ->
+  d <> b ->
+  @storeA_swap V K _ _ a b (@storeA_swap V K _ _ c d s : StoreA K) =
+  @storeA_swap V K _ _ c d (@storeA_swap V K _ _ a b s : StoreA K).
+Proof.
+  intros Hca Hcb Hda Hdb.
+  rewrite storeA_swap_conjugate.
+  rewrite (swap_fresh a b c) by congruence.
+  rewrite (swap_fresh a b d) by congruence.
+  reflexivity.
+Qed.
+
+Lemma storeA_swap_conjugate_inv {K : Type} `{Countable K}
+    (a b x y : K) (s : StoreA K) :
+   @storeA_swap V K _ _ x y (@storeA_swap V K _ _ a b s : StoreA K) =
+   @storeA_swap V K _ _ a b
+    (@storeA_swap V K _ _ (swap a b x) (swap a b y) s : StoreA K).
+Proof.
+  apply storeA_map_eq. intros z.
+  change (((@storeA_swap V K _ _ x y
+    (@storeA_swap V K _ _ a b s) : gmap K V) !! z) =
+    ((@storeA_swap V K _ _ a b
+      (@storeA_swap V K _ _ (swap a b x) (swap a b y) s) :
+      gmap K V) !! z)).
+  rewrite !storeA_swap_lookup_inv.
+  rewrite swap_conjugate. reflexivity.
+Qed.
+
+End AbstractStoreCore.
+
+Section AbstractStoreCore.
+
+Context {V : Type} `{ValueSig V}.
+
+Lemma storeA_shift_lookup {K : Type} `{Countable K} `{!ShiftKey K}
+    (k : nat) (s : StoreA K) (z : K) :
+  ((storeA_shift k s : gmap K V) !! key_shift k z) =
+  ((s : gmap K V) !! z).
+Proof.
+  unfold storeA_shift.
+  apply storeA_rekey_lookup, key_shift_inj.
+Qed.
+
+Lemma storeA_shift_dom {K : Type} `{Countable K} `{!ShiftKey K}
+    (k : nat) (s : StoreA K) :
+  dom (storeA_shift k s : gmap K V) =
+  set_map (key_shift k) (dom (s : gmap K V)).
+Proof.
+  unfold storeA_shift.
+  apply storeA_rekey_dom, key_shift_inj.
+Qed.
+
+Lemma storeA_shift_empty {K : Type} `{Countable K} `{!ShiftKey K} k :
+  storeA_shift k (∅ : StoreA K) = (∅ : gmap K V).
+Proof.
+  unfold storeA_shift.
+  apply storeA_rekey_empty.
+Qed.
+
+Lemma storeA_shift_insert {K : Type} `{Countable K} `{!ShiftKey K}
+    k z v (s : StoreA K) :
+  storeA_shift k (<[z := v]> s) =
+  <[key_shift k z := v]> (storeA_shift k s : gmap K V).
+Proof.
+  unfold storeA_shift.
+  apply storeA_rekey_insert, key_shift_inj.
+Qed.
+
+Lemma storeA_shift_union {K : Type} `{Countable K} `{!ShiftKey K}
+    k (s1 s2 : StoreA K) :
+  storeA_shift k (@union (gmap K V) _ (s1 : gmap K V) (s2 : gmap K V)) =
+  (storeA_shift k s1 : gmap K V) ∪ (storeA_shift k s2 : gmap K V).
+Proof.
+  unfold storeA_shift.
+  apply storeA_rekey_union, key_shift_inj.
+Qed.
+
+End AbstractStoreCore.
